Nearly there with allows WF_ALPHA_PREDICATE injection into vdmval.

theories/models/utp_vdm_simple/utp_vdm_sorts.thy
@@ -2,6 +2,7 @@ theory utp_vdm_sorts
 imports 
   "../../core/utp_sorts"
   "../../alpha/utp_alpha_pred" 
+  "../../alpha/utp_alpha_map" 
   utp_vdm_inject 
 begin
 
@@ -236,8 +237,6 @@ instance proof
 qed
 end
 
-
-
 lemma carrier_vcarrier [simp]: "carrier t = vcarrier (prjTYPE t)"
   by (simp add:carrier_def vcarrier_def)
 
@@ -264,89 +263,82 @@ lemma prjTYPE_vdmval_FuncT [simp]:
 done
 *)
 
-definition WF_BINDING_MAP :: "('VALUE VAR, 'VALUE) fmap set" where
-"WF_BINDING_MAP = {f. \<forall>x. x \<in>\<^sub>f fdom f \<longrightarrow> the (\<langle>f\<rangle>\<^sub>m x) \<rhd> x}"
+definition vdm_enc_var ::
+  "vdmval VAR \<Rightarrow> vbasic" where
+"vdm_enc_var v = RecI [NameI (name v), TypeI (prjTYPE (vtype v)), BoolI (aux v)]"
 
-definition binding_fmap ::
-  "'VALUE ALPHABET \<Rightarrow> 'VALUE WF_BINDING \<Rightarrow> ('VALUE VAR, 'VALUE) fmap" where
-"binding_fmap a b = list_fmap (map (\<lambda> x. (x, \<langle>b\<rangle>\<^sub>b x)) (flist a))"
+definition vdm_dec_var ::
+  "vbasic \<Rightarrow> vdmval VAR" where
+"vdm_dec_var v = 
+  (let r = the (ProjRecI v) 
+    in MkVar (the (ProjNameI (r!0))) (embTYPE (the (ProjTypeI (r!1)))) (the (ProjBoolI (r!2))))"
 
-lemma binding_fmap_rep_eq: 
-  assumes "x \<in>\<^sub>f a"
-  shows "\<langle>binding_fmap a b\<rangle>\<^sub>m x = Some (\<langle>b\<rangle>\<^sub>b x)"
+lemma vdm_enc_var_inv [simp]:
+  "vdm_dec_var (vdm_enc_var v) = v"
+  by (simp add:vdm_enc_var_def vdm_dec_var_def MkVar_def)
+
+
+definition vdm_encode_binding :: 
+  "vdmval ALPHABET \<Rightarrow> vdmval WF_BINDING \<Rightarrow> vbasic" where
+"vdm_encode_binding a b =
+  (let bf = fmap_list (binding_fmap a b)
+    in PairI (FinI (map (vdm_enc_var \<circ> fst) bf)) (ListI (map (ProjBasicV \<circ> snd) bf)))"
+
+fun vdm_decode_binding ::
+  "vbasic \<Rightarrow> vdmval WF_BINDING" where
+"vdm_decode_binding (PairI (FinI vs) (ListI bs)) = fmap_binding (list_fmap (zip (map vdm_dec_var vs) (map BasicV bs)))"
+
+lemma ProjBasicV_vbvalues_inv [simp]: 
+  "v \<in> vbvalues \<Longrightarrow> BasicV (ProjBasicV v) = v"
+  by (auto simp add:vbvalues_def)
+
+lemma 
+  assumes "\<forall>v. v \<in>\<^sub>f a \<longrightarrow> prjTYPE (vtype v) \<in> vbtypes" 
+  shows "vdm_decode_binding (vdm_encode_binding a b) \<cong> b on \<langle>a\<rangle>\<^sub>f"
 proof -
-  obtain xs where fset: "a = fset xs" and lprops: "sorted xs" "distinct xs"
-    by (metis flist_inv flist_props)
 
-  with assms have "x \<in>\<^sub>f fset xs"
-    by simp
+  have map_simp:
+        "map (BasicV \<circ> (ProjBasicV \<circ> snd)) (fmap_list (binding_fmap a b)) =
+        map snd (fmap_list (binding_fmap a b))" (is "?A = ?B")
+  proof -
+    have "?A = map (BasicV \<circ> ProjBasicV) (map snd (fmap_list (binding_fmap a b)))"
+      by (metis map_map)
 
-  with lprops have "\<langle>binding_fmap (fset xs) b\<rangle>\<^sub>m x = Some (\<langle>b\<rangle>\<^sub>b x)"
-    apply (induct xs)
-    apply (simp add: binding_fmap_def list_fmap.rep_eq)+
-    apply (subgoal_tac "flist (finsert xa (fset xs)) = (xa # flist (fset xs))")
-    apply (simp add: sorted_Cons)
-    apply (metis)
-    apply (metis (lifting) distinct.simps(2) fset_cons fset_inv sorted_Cons)
+    also have "... = map snd (fmap_list (binding_fmap a b))"
+    proof -
+      from assms have "\<forall> x \<in> set (map snd (fmap_list (binding_fmap a b))). x \<in> vbvalues"
+        apply (simp add: fmap_list_binding_fmap)
+        apply (rule ballI)
+        apply (drule_tac x="x" in spec)
+        apply (simp)
+        apply (subgoal_tac "\<langle>b\<rangle>\<^sub>b x : vtype x")
+        apply (simp)
+        apply (erule vbtypes_type_cases)
+        apply (simp add:vbvalues_def)
+        apply (simp add:vbvalues_def)
+        apply (auto)
+        apply (simp add:vbvalues_def vbtypes_def)
+        sorry
+
+      with assms show ?thesis
+        by (metis (no_types) map_idI o_def ProjBasicV_vbvalues_inv)
+    qed
+    
+    ultimately show ?thesis by simp
+
+  qed
+  
+  show ?thesis
+    apply (simp add:vdm_encode_binding_def)
+    apply (simp add:Let_def)
+    apply (simp add:map_simp)
+    apply (unfold comp_def)
+    apply (simp only: vdm_enc_var_inv zip_map_fst_snd)
+    apply (simp)
+    apply (subgoal_tac "vdm_dec_var \<circ> (vdm_enc_var \<circ> fst) = fst")
+    apply (metis binding_fmap_inv)
+    apply (simp add:comp_def)
   done
-
-  with fset show ?thesis
-    by (simp)
 qed
-
-lemma fdom_binding_map [simp]:
-  "fdom (binding_fmap a b) = a"
-  by (auto simp add:binding_fmap_def)
-
-lemma binding_fmap [closure]:
-  "binding_fmap a b \<in> WF_BINDING_MAP"
-  apply (unfold WF_BINDING_MAP_def)
-  apply (rule CollectI)
-  apply (rule allI)
-  apply (simp add:binding_fmap_rep_eq)
-done
-
-definition fmap_binding ::
-  "('VALUE VAR, 'VALUE) fmap \<Rightarrow> 'VALUE WF_BINDING" where
-"fmap_binding f = Abs_WF_BINDING (\<lambda> x. if (x \<in>\<^sub>f Fmap.fdom f) then the (\<langle>f\<rangle>\<^sub>m x) else default (vtype x))"
-
-lemma fmap_binding_rep_eq:
-  "f \<in> WF_BINDING_MAP \<Longrightarrow> 
-   \<langle>fmap_binding f\<rangle>\<^sub>b = (\<lambda> x. if (x \<in>\<^sub>f Fmap.fdom f) then the (\<langle>f\<rangle>\<^sub>m x) else default (vtype x))"
-  apply (subgoal_tac "(\<lambda> x. if (x \<in>\<^sub>f Fmap.fdom f) then the (\<langle>f\<rangle>\<^sub>m x) else default (vtype x)) \<in> WF_BINDING")
-  apply (simp add:fmap_binding_def)
-  apply (unfold WF_BINDING_def)
-  apply (unfold WF_BINDING_MAP_def)
-  apply (rule CollectI)
-  apply (rule allI)
-  apply (case_tac "v \<in>\<^sub>f fdom f")
-  apply (auto intro:typing defined)
-done
-
-lemma binding_fmap_inv:
-  "fmap_binding (binding_fmap a b) \<cong> b on \<langle>a\<rangle>\<^sub>f"
-  by (simp add:binding_equiv_def closure fmap_binding_rep_eq binding_fmap_rep_eq)
-
-definition predicate_maps :: 
-  "'VALUE ALPHABET \<Rightarrow>    'VALUE WF_PREDICATE \<Rightarrow> ('VALUE VAR, 'VALUE) fmap set" where
-"predicate_maps a p = binding_fmap a ` destPRED p"
-
-definition maps_predicate :: 
-  "('VALUE VAR, 'VALUE) fmap set \<Rightarrow> 'VALUE WF_PREDICATE" where
-"maps_predicate fs = mkPRED {b. \<exists>f\<in>fs. fmap_binding f \<cong> b on \<langle>fdom f\<rangle>\<^sub>f}"
-
-lemma predicate_maps_inv[simp]:
-  "maps_predicate (predicate_maps (\<alpha> p) (\<pi> p)) = \<pi> p"
-  apply (simp add:maps_predicate_def predicate_maps_def)
-  apply (subgoal_tac "\<And> b f. (fmap_binding (binding_fmap (\<alpha> p) f) \<cong> b on \<langle>\<alpha> p\<rangle>\<^sub>f) = f \<cong> b on \<langle>\<alpha> p\<rangle>\<^sub>f")
-  apply (safe)
-  apply (smt UNIV_I WF_ALPHA_PREDICATE_binding_equiv mem_Collect_eq mkPRED_inverse)
-  apply (simp)
-  apply (rule_tac x="x" in bexI)
-  apply (metis binding_fmap_inv)
-  apply (simp)
-  apply (metis (lifting) binding_equiv_comm binding_equiv_trans binding_fmap_inv)
-  apply (metis (lifting) binding_equiv_trans binding_fmap_inv)
-done
 
 end
